Simple_Clause_Learning/Initial_Literals_Generalize_Learned_Literals.thy
@@ -292,13 +292,13 @@ lemma backtrack_initial_lits_generalized_learned_lits:
   "backtrack N \<beta> S S' \<Longrightarrow> initial_lits_generalized_learned_lits N S \<Longrightarrow>
     initial_lits_generalized_learned_lits N S'"
 proof (induction S S' rule: backtrack.induct)
-  case (backtrackI \<Gamma> D \<sigma> L U)
+  case (backtrackI \<Gamma> \<Gamma>' D \<sigma> L U)
   then show ?case
     unfolding initial_lits_generalized_learned_lits_def
     apply simp
-    by (smt (verit, best) Un_assoc Un_commute Un_insert_left
-        clss_lits_generalize_clss_lits_if_superset clss_lits_generalize_clss_lits_trans
-        clss_of_trail_trail_decide_subset sup.absorb_iff1 sup.right_idem)
+    by (metis (no_types, opaque_lifting) Un_assoc clss_lits_generalize_clss_lits_insert
+        clss_lits_generalize_clss_lits_subset clss_of_trail_trail_decide
+        clss_of_trail_trail_decide_subset subset_Un_eq sup_ge1)
 qed
 
 abbreviation lits_of_clss where
